Proof of no aborts in validator_set::derive_reference_gas_price

crates/sui-framework/packages/sui-system/sources/other_specs.move
@@ -4,7 +4,9 @@
 module sui_system::other_specs;
 
 use sui::tx_context::TxContext;
-use std::option::{Option,some,none};
+use sui::priority_queue;
+use std::u64;
+
 use prover::prover::{drop,ensures,requires,val};
 
 #[spec(target=sui::tx_context::epoch)]
@@ -15,6 +17,12 @@ public fun epoch_spec(self: &TxContext): u64 {
 #[spec(target=sui::tx_context::sender)]
 public fun sender_spec(self: &TxContext): address {
     sui::tx_context::sender(self)
+}
+
+#[spec(target=sui::priority_queue::new)]
+public fun new_spec<T: drop>(mut entries: vector<priority_queue::Entry<T>>): priority_queue::PriorityQueue<T> {
+    requires(entries.length() < u64::max_value!() - 1);
+    priority_queue::new(entries)
 }
 
 #[spec(target=std::option::destroy_some)] // see sui-prover issue #144
